theories/ordinals/Ackermann/folProp.v
@@ -20,7 +20,6 @@ Let apply := apply L.
 Let equal := equal L.
 Let atomic := atomic L.
 
-Let notH := notH L.
 Let forallH := forallH L.
 Let lt_depth := lt_depth L.
 
